Writing CompileModule2

platform/cito/CompileModule2.v
@@ -1,13 +1,5 @@
 Set Implicit Arguments.
 
-Require Import Arith.
-Open Scope nat_scope.
-
-Require Import GoodModule.
-Local Notation MName := Name.
-Require Import GLabelMap.
-Require Import StringMap.
-
 Require Import ADT.
 
 Module Make (Import E : ADT).
@@ -24,27 +16,39 @@ Module Make (Import E : ADT).
   Require Import LinkSpec.
   Import LinkSpecMake.
 
+  Require Import GLabelMap.
+  Require Import StringMap.
+  Require Import CModule.
+
   Section M.
 
-    Variable m : GoodModule.
+    Variable m : CModule.
     
     Variable imports : GLabelMap.t ForeignFuncSpec.
 
-    Definition modules := m :: nil.
-
     Variable exports : StringMap.t ForeignFuncSpec.
 
-    Definition m_name := MName m.
+    (* the name of the module that contains axiomatic export specs *)
+    Variable ax_mod_name : string.
+
+    (* the name of the module that contains operational export specs *)
+    Variable op_mod_name : string.
+
+    Hypothesis op_mod_name_ok : is_good_module_name op_mod_name = true.
+
+    Definition cmod := cmodule_to_gmodule op_mod_name op_mod_name_ok m.
+
+    Definition modules := cmod :: nil.
 
     Arguments GLabelMap.empty {elt}.
 
-    Definition aug_mod_name elt (m : StringMap.t elt) := StringMap.fold (fun k v a => GLabelMap.add (m_name, k) v a) m GLabelMap.empty.
+    Definition aug_mod_name elt m_name (m : StringMap.t elt) := StringMap.fold (fun k v a => GLabelMap.add (m_name, k) v a) m GLabelMap.empty.
 
-    Definition exports' := aug_mod_name exports.
     Definition specs_op := make_specs modules imports.
-    Definition specs := apply_specs_diff specs_op exports'.
+    Definition exports_with_glabel := aug_mod_name ax_mod_name exports.
+    Definition specs := apply_specs_diff specs_op exports_with_glabel.
 
-    Hypothesis specs_strengthen_diff : forall env_ax, specs_env_agree specs env_ax -> strengthen_diff specs_op exports' env_ax.
+    Hypothesis specs_strengthen_diff : forall env_ax, specs_env_agree specs env_ax -> strengthen_diff specs_op exports_with_glabel env_ax.
 
     Lemma specs_op_equal : specs_equal specs_op modules imports.
       admit.
@@ -80,29 +84,36 @@ Module Make (Import E : ADT).
 
     Section M.
 
-      Variable new_m_name : string.
-
-      Variable m : GoodModule.
+      Variable m : CModule.
       
-      Definition old_m_name := MName m.
-
-      Definition modules := m :: nil.
-
       Variable imports : GLabelMap.t ForeignFuncSpec.
 
       Variable exports : StringMap.t ForeignFuncSpec.
 
+      Variable ax_mod_name : string.
+
+      Variable op_mod_name : string.
+
+      Hypothesis op_mod_name_ok : is_good_module_name op_mod_name = true.
+
+      Definition cmod := cmodule_to_gmodule op_mod_name op_mod_name_ok m.
+
+      Definition modules := cmod :: nil.
+
+      Definition tgt_spec name f := func_spec modules imports (op_mod_name, name) f.
+
       Require Import StringMapFacts.
 
-      Definition accessible_labels := List.map (fun l => (old_m_name, l)) (StringMapFacts.keys exports).
+      Definition accessible_labels := 
+        List.map (fun fname => (op_mod_name, fname)) (StringMapFacts.keys exports).
 
       Section Fun.
 
-        Variable f : GoodFunction.
-
-        Definition fname := Name f.
+        Variable fname : string.
 
         Variable spec : ForeignFuncSpec.
+
+        Variable f : CFun.
 
         Section body.
           
@@ -112,31 +123,45 @@ Module Make (Import E : ADT).
 
           Variable im_g : importsGlobal im.
 
-          Definition tgt : glabel := (old_m_name, fname).
-
-          Definition tgt_spec := func_spec modules imports (old_m_name, fname) f.
+          Definition tgt : glabel := (op_mod_name, fname).
 
           Definition body := 
-            @Seq_ _ im_g new_m_name
-                  (AssertStar_ im new_m_name accessible_labels tgt_spec)
-                  (Goto_ im_g new_m_name tgt).
+            @Seq_ _ im_g ax_mod_name
+                  (AssertStar_ im ax_mod_name accessible_labels (tgt_spec fname f))
+                  (Goto_ im_g ax_mod_name tgt).
 
         End body.
 
-        Definition new_spec := foreign_func_spec (new_m_name, fname) spec.
+        Definition stub_spec := foreign_func_spec (ax_mod_name, fname) spec.
 
-        Definition make_stub : StructuredModule.function new_m_name :=
-          (fname, new_spec, body).
+        Definition make_stub : StructuredModule.function ax_mod_name :=
+          (fname, stub_spec, body).
 
       End Fun.
-      
-      Definition select_funs m names := 
-        match names
-      Definition bimports : list import := List.map tgt_spec (select_funs m (keys exports)).
-      
-      Definition stubs := List.map make_stub (Functions m).
 
-      Definition make_module := StructuredModule.bmodule_ bimports_diff_bexports stubs.
+      Import StringMap.
+
+      Arguments StringMap.empty {elt}.
+
+      Definition inter elt1 elt2 (d1 : t elt1) (d2 : t elt2) := fold (fun k v1 acc => match find k d2 with | Some v2 => add k (v1, v2) acc | None => acc end) d1 empty.
+
+      Definition content := inter exports (Funs m).
+
+      Definition tgt_spec_as_import {unused} (x : string * (unused * CFun)) : import := 
+        match x with (name, (_, f)) => (op_mod_name, name, tgt_spec name f) end.
+
+      Definition bimports : list import := List.map tgt_spec_as_import (elements content).
+      
+      Definition stubs := List.map (fun x => match x with (name, (ax, op)) => make_stub name ax op end) (elements content).
+
+      Definition make_module := StructuredModule.bmodule_ bimports stubs.
+
+      Theorem make_module_ok : XCAP.moduleOk make_module.
+        eapply bmoduleOk.
+        eapply module_name_not_in_imports.
+        eapply no_dup_func_names.
+        eapply good_vcs; eauto.
+      Qed.
 
 
 (*
